Теорема
	Пусть
		 $\left. \begin{array}{l} 1)\lim_{ x \to a }f(x)=A \\ 2)\lim_{ x \to a }g(x)=B \\ 3)\exists \dot{\cup}(a),\text{ в которой }f(x)\leq g(x) \end{array} \right\}\implies A\leq B$
Док-во
	Пусть $\{ x_{n} \}\underset{ n\to \infty }{ \to } a,x_{n}\neq a,n\in \mathbf{N}\implies \exists N:\forall n>N\implies x_{n}\in \dot{\cup}(a)\implies\forall n>N\implies f(x_{n})\leq g(x_{n})\implies A\leq B\text{ т.к. }\lim_{ n \to \infty }f(x_{n})=A\text{ и }\lim_{ n \to \infty }g(x_{n})=B$
Теорема (о промежуточных значениях)
	Пусть
		1) $\exists \lim_{ x \to a }f_{1}(x)=A=\lim_{ x \to a }f_{2}(x)$
		2) $\exists \dot{\cup}(a)\text{, в которой }f_{1}(x)\leq g(x)\leq f_{2}(x)$
	Тогда
		$\exists \lim_{ x \to a }g(x)=A$
Док-во
	Пусть произв. $\{ x_{n} \}\to a,x_{n}\neq a,n\in \mathbf{N}\implies \exists N:\forall n>N\implies x_{n}\in \dot{\cup}(a)\implies\forall n>N\implies f_{1}(x_{n})\leq g(x_{n})\leq f_{2}(x_{n})\implies \exists \lim_{ n \to \infty }g(x_{n})=A\text{, т.к. }\exists \lim_{ n \to \infty }f_{1}(x_{n})=A=\lim_{ n \to \infty }f_{2}(x_{n})$
	